deleted nonempty condition for defender sim answer, renamed ZR and some other lemmas

Contrasim_Set_Game.thy
@@ -20,7 +20,7 @@ fun (in lts_tau) c_set_game_moves ::
 
   simulation_answer:                        
     \<open>c_set_game_moves (DefenderSimNode a p1 Q) (AttackerNode p10 Q1) =   
-      (p1 = p10 \<and> Q1 = dsuccs a Q \<and> Q1 \<noteq> {})\<close> |                                             
+      (p1 = p10 \<and> Q1 = dsuccs a Q)\<close> |                                             
 
   swap_challenge:
     \<open>c_set_game_moves (AttackerNode p Q) (DefenderSwapNode p1 Q0) =
@@ -49,16 +49,16 @@ for
   initial :: \<open>('s, 'a) c_set_game_node\<close> 
 begin
 
-fun strategy_from_ZR_C :: \<open>('s \<Rightarrow> ('s set) \<Rightarrow> bool) \<Rightarrow> ('s, 'a) c_set_game_node strategy\<close>
+fun strategy_from_F_of_C :: \<open>('s \<Rightarrow> ('s set) \<Rightarrow> bool) \<Rightarrow> ('s, 'a) c_set_game_node strategy\<close>
   where
 
-  \<open>strategy_from_ZR_C R ((DefenderSwapNode p1 Q)#play) = 
+  \<open>strategy_from_F_of_C R ((DefenderSwapNode p1 Q)#play) = 
     (AttackerNode (SOME q1 . (\<exists>q. (q \<in> Q \<and> q  \<Rightarrow>^\<tau> q1)) \<and> R q1 {p1}) {p1})\<close> |
 
-  \<open>strategy_from_ZR_C R ((DefenderSimNode a p1 Q)#play) = 
+  \<open>strategy_from_F_of_C R ((DefenderSimNode a p1 Q)#play) = 
     (AttackerNode p1 (SOME Q1 . Q1 = dsuccs a Q \<and> R p1 Q1 \<and> Q1 \<noteq> {}))\<close> |
  
-  \<open>strategy_from_ZR_C _ _ = undefined\<close>
+  \<open>strategy_from_F_of_C _ _ = undefined\<close>
 
 lemma set_defender_pred_is_attacker: 
   assumes 
@@ -123,37 +123,37 @@ next
   then show ?thesis using DefenderSwapNode by auto
 qed
 
-lemma set_game_all_f_consistent_atk_pos_in_ZR:
+lemma set_game_strategy_retains_F:
   assumes
     \<open>contrasim C\<close>
     \<open>C p0 q0\<close>
     \<open>initial = AttackerNode p0 {q0}\<close>
-    \<open>play \<in> plays_for_strategy (strategy_from_ZR_C (ZR (set_type C)))\<close>
-  shows \<open>n = AttackerNode p Q \<Longrightarrow> n \<in> set play \<Longrightarrow> ZR (set_type C) p Q \<close>
+    \<open>play \<in> plays_for_strategy (strategy_from_F_of_C (F (set_type C)))\<close>
+  shows \<open>n = AttackerNode p Q \<Longrightarrow> n \<in> set play \<Longrightarrow> F (set_type C) p Q \<close>
 proof (induct arbitrary: n p Q rule: plays_for_strategy.induct[OF assms(4)])
   case init: 1
   hence \<open>n = initial\<close> by auto
   hence \<open>p = p0 \<and> Q = {q0}\<close> using assms(3) init.prems(1) by auto 
-  thus  \<open>ZR (set_type C) p Q\<close> using assms R_is_in_ZR set_type_def by simp
+  thus  \<open>F (set_type C) p Q\<close> using assms R_is_in_F_of_R set_type_def by simp
 next
   case p0moved: (2 n0 play) 
-  hence \<open>(n = strategy_from_ZR_C (ZR (set_type C)) (n0 # play)) \<or> (n \<in> set (n0#play))\<close> by auto
+  hence \<open>(n = strategy_from_F_of_C (F (set_type C)) (n0 # play)) \<or> (n \<in> set (n0#play))\<close> by auto
   thus ?case
   proof(rule disjE)
     assume \<open>n \<in> set (n0#play)\<close>
     thus ?thesis using p0moved.prems p0moved.hyps(1,2) by blast 
   next
-    assume strat: \<open>n = strategy_from_ZR_C (ZR (set_type C)) (n0 # play)\<close>
+    assume strat: \<open>n = strategy_from_F_of_C (F (set_type C)) (n0 # play)\<close>
     hence \<open>(\<exists>a Qpred. n0 = DefenderSimNode a p Qpred) \<or> (\<exists>q Ppred. n0 = DefenderSwapNode q Ppred \<and> Q = {q})\<close>
       using def_sim_or_swap_before_atkNode[OF p0moved.hyps(4), of \<open>p\<close> \<open>Q\<close>] p0moved.prems(1) by blast 
     thus ?case 
     proof (rule disjE)
       assume \<open>\<exists>a Qpred. n0 = DefenderSimNode a p Qpred\<close>
       then obtain a Qpred where n0_def: \<open>n0 = DefenderSimNode a p Qpred\<close> by auto
-      hence \<open>strategy_from_ZR_C (ZR (set_type C)) (n0#play) 
-          = AttackerNode p (SOME Q1. Q1 = dsuccs a Qpred \<and> (ZR (set_type C)) p Q1 \<and> Q1 \<noteq> {})\<close> 
-        using strategy_from_ZR_C.simps(2) by auto
-      hence Q_def: \<open>Q = (SOME Q1. Q1 = dsuccs a Qpred \<and> (ZR (set_type C)) p Q1  \<and> Q1 \<noteq> {})\<close> 
+      hence \<open>strategy_from_F_of_C (F (set_type C)) (n0#play) 
+          = AttackerNode p (SOME Q1. Q1 = dsuccs a Qpred \<and> (F (set_type C)) p Q1 \<and> Q1 \<noteq> {})\<close> 
+        using strategy_from_F_of_C.simps(2) by auto
+      hence Q_def: \<open>Q = (SOME Q1. Q1 = dsuccs a Qpred \<and> (F (set_type C)) p Q1  \<and> Q1 \<noteq> {})\<close> 
         using strat by (simp add: p0moved.prems(1))
       have \<open>\<exists>ppred. hd play = (AttackerNode ppred Qpred) \<and> c_set_game_moves (hd play) n0\<close> 
         using set_defender_pred_is_attacker strategy_plays_subset[OF p0moved.hyps(1)] 
@@ -164,21 +164,21 @@ next
       hence \<open>hd play \<in> set (n0 # play)\<close> 
         using second_elem_in_play_set strategy_plays_subset[OF p0moved.hyps(1)] assms(3) n0_def
         by (simp add: assms(4))
-      hence \<open>ZR (set_type C) ppred Qpred\<close> using p0moved.hyps(2) ppred_def by blast
-      hence \<open>dsuccs a Qpred \<noteq> {} \<and> ZR (set_type C) p (dsuccs a Qpred)\<close> 
-       using \<open>ppred =\<rhd>a p\<close> assms(1,2,4) ZR_C_guarantees_action_succ \<open>a \<noteq> \<tau>\<close> by auto
-      hence \<open>\<exists>Q. Q = (dsuccs a Qpred) \<and> ZR (set_type C) p Q\<close> by auto
-      from someI_ex[OF this] show \<open>ZR (set_type C) p Q\<close> 
+      hence \<open>F (set_type C) ppred Qpred\<close> using p0moved.hyps(2) ppred_def by blast
+      hence \<open>dsuccs a Qpred \<noteq> {} \<and> F (set_type C) p (dsuccs a Qpred)\<close> 
+       using \<open>ppred =\<rhd>a p\<close> assms(1,2,4) F_of_C_guarantees_action_succ \<open>a \<noteq> \<tau>\<close> by auto
+      hence \<open>\<exists>Q. Q = (dsuccs a Qpred) \<and> F (set_type C) p Q\<close> by auto
+      from someI_ex[OF this] show \<open>F (set_type C) p Q\<close> 
         unfolding Q_def
         using n0_def p0moved.hyps(4) by auto
     next
       assume \<open>(\<exists>q Ppred. n0 = DefenderSwapNode q Ppred \<and> Q = {q})\<close>
       then obtain q Ppred where n0_def: \<open>n0 = DefenderSwapNode q Ppred\<close> and Q_def: \<open>Q = {q}\<close> 
         by auto
-      hence \<open>strategy_from_ZR_C (ZR (set_type C)) (n0#play)
-         = AttackerNode (SOME p1. (\<exists>p. p \<in> Ppred \<and> p \<Rightarrow>^\<tau> p1) \<and> (ZR (set_type C)) p1 {q}) {q}\<close> 
-        using strategy_from_ZR_C.simps(1) by auto
-      hence p_def: \<open>p = (SOME p1. (\<exists>p. p \<in> Ppred \<and> p \<Rightarrow>^\<tau> p1) \<and> (ZR (set_type C)) p1 {q})\<close> 
+      hence \<open>strategy_from_F_of_C (F (set_type C)) (n0#play)
+         = AttackerNode (SOME p1. (\<exists>p. p \<in> Ppred \<and> p \<Rightarrow>^\<tau> p1) \<and> (F (set_type C)) p1 {q}) {q}\<close> 
+        using strategy_from_F_of_C.simps(1) by auto
+      hence p_def: \<open>p = (SOME p1. (\<exists>p. p \<in> Ppred \<and> p \<Rightarrow>^\<tau> p1) \<and> (F (set_type C)) p1 {q})\<close> 
         using strat p0moved.prems by auto
       have \<open>\<exists>qpred. hd play = (AttackerNode qpred Ppred) \<and> c_set_game_moves (hd play) n0\<close> 
         using set_defender_pred_is_attacker strategy_plays_subset[OF p0moved.hyps(1)] 
@@ -191,13 +191,13 @@ next
       have \<open>hd play \<in> set (n0 # play)\<close> 
         using second_elem_in_play_set strategy_plays_subset[OF p0moved.hyps(1)] assms(3) n0_def
         by (simp add: assms(4)) 
-      hence \<open>ZR (set_type C) qpred Ppred\<close> using p0moved.hyps(2) qpred_def by blast
-      hence \<open>\<exists>p. p \<in> weak_tau_succs Ppred \<and> ZR (set_type C) p {q}\<close> 
-        using qpred_q_move assms(1,2) ZR_C_guarantees_tau_succ by blast
-      hence \<open>\<exists>p. (\<exists>p0. p0 \<in> Ppred \<and> p0 \<Rightarrow>^\<tau>  p) \<and> ZR (set_type C) p {q}\<close> 
+      hence \<open>F (set_type C) qpred Ppred\<close> using p0moved.hyps(2) qpred_def by blast
+      hence \<open>\<exists>p. p \<in> weak_tau_succs Ppred \<and> F (set_type C) p {q}\<close> 
+        using qpred_q_move assms(1,2) F_of_C_guarantees_tau_succ by blast
+      hence \<open>\<exists>p. (\<exists>p0. p0 \<in> Ppred \<and> p0 \<Rightarrow>^\<tau>  p) \<and> F (set_type C) p {q}\<close> 
         using weak_tau_succs_def[of \<open>Ppred\<close>] by blast
-      from someI_ex[OF this] p_def have \<open>ZR (set_type C) p {q}\<close> by simp
-      thus \<open>ZR (set_type C) p Q\<close> using Q_def by blast
+      from someI_ex[OF this] p_def have \<open>F (set_type C) p {q}\<close> by simp
+      thus \<open>F (set_type C) p Q\<close> using Q_def by blast
     qed
   qed
 next  
@@ -222,11 +222,11 @@ lemma set_contrasim_game_complete:
     \<open>contrasim C\<close>
     \<open>C p0 q0\<close>
     \<open>initial = AttackerNode p0 {q0}\<close>
-  shows \<open>player0_winning_strategy (strategy_from_ZR_C (ZR (set_type C)))\<close>
+  shows \<open>player0_winning_strategy (strategy_from_F_of_C (F (set_type C)))\<close>
   unfolding player0_winning_strategy_def
 proof (safe)
   fix play
-  assume A1: \<open>play \<in> (plays_for_strategy (strategy_from_ZR_C (ZR (set_type C))))\<close>
+  assume A1: \<open>play \<in> (plays_for_strategy (strategy_from_F_of_C (F (set_type C))))\<close>
   thus \<open>player1_wins play \<Longrightarrow> False\<close>
     unfolding player1_wins_def
   proof - 
@@ -242,11 +242,11 @@ proof (safe)
       from p0moved.hyps have \<open>c_set_game_defender_node n0\<close> by simp
       hence \<open>(\<exists>a p1 q. n0 = (DefenderSimNode a p1 q)) \<or> (\<exists>q P. n0 = DefenderSwapNode q P)\<close>
         by (meson c_set_game_defender_node.elims(2)) 
-      hence \<open>\<not>c_set_game_defender_node (strategy_from_ZR_C (ZR (set_type C)) (n0#play))\<close>
+      hence \<open>\<not>c_set_game_defender_node (strategy_from_F_of_C (F (set_type C)) (n0#play))\<close>
         using p0moved.hyps(4) 
-          c_set_game_moves.elims(2)[of \<open>n0\<close> \<open>strategy_from_ZR_C (ZR (set_type C)) (n0#play)\<close>]
+          c_set_game_moves.elims(2)[of \<open>n0\<close> \<open>strategy_from_F_of_C (F (set_type C)) (n0#play)\<close>]
         by force 
-      hence \<open>\<not>c_set_game_defender_node (hd (strategy_from_ZR_C (ZR (set_type C)) (n0 # play) # n0 # play))\<close> 
+      hence \<open>\<not>c_set_game_defender_node (hd (strategy_from_F_of_C (F (set_type C)) (n0 # play) # n0 # play))\<close> 
         by simp
       hence \<open>False\<close> using p0moved.prems ..
       then show ?case ..
@@ -255,8 +255,8 @@ proof (safe)
       hence \<open>\<not>c_set_game_defender_node n1\<close> using p1moved.hyps and player1_position_def by simp
       then obtain p Q where n1_def: \<open>n1 = AttackerNode p Q\<close>
         using c_set_game_defender_node.elims(3) by auto
-      hence ZR: \<open>ZR (set_type C) p Q\<close> 
-        using set_game_all_f_consistent_atk_pos_in_ZR[OF assms(1-3), of \<open>n1#play\<close>, OF p1moved.hyps(1)] 
+      hence in_F: \<open>F (set_type C) p Q\<close> 
+        using set_game_strategy_retains_F[OF assms(1-3), of \<open>n1#play\<close>, OF p1moved.hyps(1)] 
         by auto
       have \<open>(\<exists>a p1. n1' = DefenderSimNode a p1 Q) \<or> (\<exists>p1. n1' = DefenderSwapNode p1 Q)\<close> 
         using p1moved.prems n1_def p1moved.hyps(4)
@@ -269,10 +269,10 @@ proof (safe)
           using p1moved.hyps n1_def n1'_def by auto
         hence \<open>p =\<rhd>a p1\<close> by auto
         hence \<open>p \<Rightarrow>^a p1\<close> using steps.refl by blast 
-        hence \<open>dsuccs a Q \<noteq> {} \<and> ZR (set_type C) p1 (dsuccs a Q)\<close> 
-          using ZR_C_guarantees_action_succ move
-          by (metis ZR assms(1) simulation_challenge tau_tau) 
-        then obtain Q1 where \<open>Q1 = dsuccs a Q \<and> ZR (set_type C) p1 Q1 \<and> Q1 \<noteq> {}\<close> by blast
+        hence \<open>dsuccs a Q \<noteq> {} \<and> F (set_type C) p1 (dsuccs a Q)\<close> 
+          using F_of_C_guarantees_action_succ move
+          by (metis in_F assms(1) simulation_challenge tau_tau) 
+        then obtain Q1 where \<open>Q1 = dsuccs a Q \<and> F (set_type C) p1 Q1 \<and> Q1 \<noteq> {}\<close> by blast
         hence \<open>c_set_game_moves n1' (AttackerNode p1 Q1)\<close> 
           using A n1'_def by auto
         thus \<open>\<exists>a. c_set_game_moves (hd (n1' # n1 # play)) a\<close> by auto
@@ -282,9 +282,9 @@ proof (safe)
         hence \<open>c_set_game_moves (AttackerNode p Q) (DefenderSwapNode p1 Q)\<close> 
           using p1moved.hyps(4) n1_def by auto
         hence p_succ: \<open>p \<Rightarrow>^\<tau> p1\<close> by auto
-        hence \<open>\<exists>q'. q' \<in> weak_tau_succs Q \<and> ZR (set_type C) q' {p1}\<close> 
-          using ZR ZR_C_guarantees_tau_succ assms(1) by auto
-        hence \<open>\<exists>q1. q1 \<in> weak_tau_succs Q \<and> ZR (set_type C) q1 {p1}\<close> by auto
+        hence \<open>\<exists>q'. q' \<in> weak_tau_succs Q \<and> F (set_type C) q' {p1}\<close> 
+          using in_F F_of_C_guarantees_tau_succ assms(1) by auto
+        hence \<open>\<exists>q1. q1 \<in> weak_tau_succs Q \<and> F (set_type C) q1 {p1}\<close> by auto
         hence \<open>\<exists>q1 P1. c_set_game_moves n1' (AttackerNode q1 P1)\<close> using n1'_def  by auto  
         thus \<open>\<exists>a. c_set_game_moves (hd (n1' # n1 # play)) a\<close> by auto
       qed
@@ -300,16 +300,16 @@ lemma strategy_from_delay_set_contrasim_sound :
     \<open>C p0 q0\<close>
     \<open>initial = AttackerNode p0 {q0}\<close>
   shows
-    \<open>sound_strategy (strategy_from_ZR_C (ZR (set_type C)))\<close>
+    \<open>sound_strategy (strategy_from_F_of_C (F (set_type C)))\<close>
   unfolding sound_strategy_def
 proof (safe)
   fix n0 play
   assume A: 
-    \<open>n0 # play \<in> plays_for_strategy (strategy_from_ZR_C (ZR (set_type C)))\<close>
+    \<open>n0 # play \<in> plays_for_strategy (strategy_from_F_of_C (F (set_type C)))\<close>
     \<open>c_set_game_defender_node n0\<close>
   hence \<open>(\<exists>a p' Q. n0 = DefenderSimNode a p' Q) \<or> (\<exists>p' Q. n0 = DefenderSwapNode p' Q)\<close>
     by (meson c_set_game_defender_node.elims(2)) 
-  thus \<open>c_set_game_moves n0 (strategy_from_ZR_C (ZR (set_type C)) (n0 # play))\<close>
+  thus \<open>c_set_game_moves n0 (strategy_from_F_of_C (F (set_type C)) (n0 # play))\<close>
   proof(rule disjE)
     assume \<open>\<exists>a p' Q. n0 = DefenderSimNode a p' Q\<close>
     then obtain a p' Q where n0_def: \<open>n0 = DefenderSimNode a p' Q\<close> by auto
@@ -318,23 +318,23 @@ proof (safe)
     hence \<open>c_set_game_moves (AttackerNode p Q) (DefenderSimNode a p' Q)\<close>
       by (metis A n0_def assms(3) set_defender_pred_is_attacker strategy_plays_subset) 
     hence \<open>p =\<rhd>a p'\<close> \<open>\<not> tau a\<close> by auto   
-    hence \<open>ZR (set_type C) p Q\<close>
-      using set_game_all_f_consistent_atk_pos_in_ZR[OF assms] A p_def
+    hence \<open>F (set_type C) p Q\<close>
+      using set_game_strategy_retains_F[OF assms] A p_def
         assms(3) second_elem_in_play_set strategy_plays_subset 
       by fastforce
-    hence  \<open>dsuccs a Q \<noteq> {} \<and> ZR (set_type C) p' (dsuccs a Q)\<close>
-      using ZR_C_guarantees_action_succ \<open>\<not> tau a\<close> \<open>p =\<rhd>a p'\<close> assms(1) tau_tau by blast 
-    hence Q1_ex: \<open>\<exists>Q'. Q' = dsuccs a Q \<and> ZR (set_type C) p' Q' \<and> Q' \<noteq> {}\<close> by auto
-    from n0_def have st: \<open>strategy_from_ZR_C (ZR (set_type C)) (n0#play) = 
-    (AttackerNode p' (SOME Q1 . Q1 = dsuccs a Q \<and> (ZR (set_type C)) p' Q1 \<and> Q1 \<noteq> {}))\<close> by auto
+    hence  \<open>dsuccs a Q \<noteq> {} \<and> F (set_type C) p' (dsuccs a Q)\<close>
+      using F_of_C_guarantees_action_succ \<open>\<not> tau a\<close> \<open>p =\<rhd>a p'\<close> assms(1) tau_tau by blast 
+    hence Q1_ex: \<open>\<exists>Q'. Q' = dsuccs a Q \<and> F (set_type C) p' Q' \<and> Q' \<noteq> {}\<close> by auto
+    from n0_def have st: \<open>strategy_from_F_of_C (F (set_type C)) (n0#play) = 
+    (AttackerNode p' (SOME Q1 . Q1 = dsuccs a Q \<and> (F (set_type C)) p' Q1 \<and> Q1 \<noteq> {}))\<close> by auto
     then obtain Q1 where 
-      \<open>AttackerNode p' (SOME Q1 . Q1 = dsuccs a Q \<and> (ZR (set_type C)) p' Q1  \<and> Q1 \<noteq> {}) = AttackerNode p' Q1\<close>
+      \<open>AttackerNode p' (SOME Q1 . Q1 = dsuccs a Q \<and> (F (set_type C)) p' Q1  \<and> Q1 \<noteq> {}) = AttackerNode p' Q1\<close>
       by blast
-    hence Q1_def: \<open>Q1 = (SOME Q1 . Q1 = dsuccs a Q \<and> (ZR (set_type C)) p' Q1 \<and> Q1 \<noteq> {})\<close>
+    hence Q1_def: \<open>Q1 = (SOME Q1 . Q1 = dsuccs a Q \<and> (F (set_type C)) p' Q1 \<and> Q1 \<noteq> {})\<close>
       by auto
-    have next_is_atk: \<open>strategy_from_ZR_C (ZR (set_type C)) (n0#play) = (AttackerNode p' Q1)\<close> 
+    have next_is_atk: \<open>strategy_from_F_of_C (F (set_type C)) (n0#play) = (AttackerNode p' Q1)\<close> 
       using st Q1_def by auto
-    with someI_ex[OF Q1_ex] Q1_def have mov_cond: \<open>Q1 = dsuccs a Q \<and> ZR (set_type C) p' Q1 \<and> Q1 \<noteq> {}\<close>
+    with someI_ex[OF Q1_ex] Q1_def have mov_cond: \<open>Q1 = dsuccs a Q \<and> F (set_type C) p' Q1 \<and> Q1 \<noteq> {}\<close>
       by blast
     have \<open>c_set_game_moves n0 (AttackerNode p' Q1)\<close> using n0_def mov_cond by auto
     thus ?thesis using next_is_atk by auto
@@ -346,22 +346,22 @@ proof (safe)
     hence \<open>c_set_game_moves (AttackerNode p Q) (DefenderSwapNode p' Q)\<close>
       by (metis A n0_def assms(3) set_defender_pred_is_attacker strategy_plays_subset)
     hence \<open>p \<Rightarrow>^\<tau> p'\<close> by auto
-    hence \<open>ZR (set_type C) p Q\<close>
-      using set_game_all_f_consistent_atk_pos_in_ZR[OF assms] A p_def
+    hence \<open>F (set_type C) p Q\<close>
+      using set_game_strategy_retains_F[OF assms] A p_def
         assms(3) second_elem_in_play_set strategy_plays_subset 
       by fastforce 
-    hence  \<open>\<exists>q'. q' \<in> weak_tau_succs Q \<and> ZR (set_type C) q' {p'}\<close>
-      using ZR_C_guarantees_tau_succ \<open>p \<Rightarrow>^\<tau> p'\<close> assms(1) by auto 
-    hence q1_ex: \<open>\<exists>q1. (\<exists>q.(q \<in> Q \<and> q  \<Rightarrow>^\<tau> q1)) \<and> ZR (set_type C) q1 {p'}\<close> using weak_tau_succs_def by auto
-    hence strat: \<open>strategy_from_ZR_C (ZR (set_type C)) (n0#play) = 
-    AttackerNode (SOME q1 . (\<exists>q. (q \<in> Q \<and> q  \<Rightarrow>^\<tau> q1)) \<and> (ZR (set_type C)) q1 {p'}) {p'}\<close>
+    hence  \<open>\<exists>q'. q' \<in> weak_tau_succs Q \<and> F (set_type C) q' {p'}\<close>
+      using F_of_C_guarantees_tau_succ \<open>p \<Rightarrow>^\<tau> p'\<close> assms(1) by auto 
+    hence q1_ex: \<open>\<exists>q1. (\<exists>q.(q \<in> Q \<and> q  \<Rightarrow>^\<tau> q1)) \<and> F (set_type C) q1 {p'}\<close> using weak_tau_succs_def by auto
+    hence strat: \<open>strategy_from_F_of_C (F (set_type C)) (n0#play) = 
+    AttackerNode (SOME q1 . (\<exists>q. (q \<in> Q \<and> q  \<Rightarrow>^\<tau> q1)) \<and> (F (set_type C)) q1 {p'}) {p'}\<close>
       using n0_def by auto
     then obtain q1 where 
-      \<open>AttackerNode (SOME q1 . (\<exists>q. (q \<in> Q \<and> q  \<Rightarrow>^\<tau> q1)) \<and> (ZR (set_type C)) q1 {p'}) {p'}
+      \<open>AttackerNode (SOME q1 . (\<exists>q. (q \<in> Q \<and> q  \<Rightarrow>^\<tau> q1)) \<and> (F (set_type C)) q1 {p'}) {p'}
       = AttackerNode q1 {p'}\<close> by blast
-    hence q1_def: \<open>q1 = (SOME q1 . (\<exists>q. (q \<in> Q \<and> q  \<Rightarrow>^\<tau> q1)) \<and> (ZR (set_type C)) q1 {p'})\<close>
+    hence q1_def: \<open>q1 = (SOME q1 . (\<exists>q. (q \<in> Q \<and> q  \<Rightarrow>^\<tau> q1)) \<and> (F (set_type C)) q1 {p'})\<close>
       by auto
-    with someI_ex[OF q1_ex] have X: \<open>\<exists>q. (q \<in> Q \<and> q  \<Rightarrow>^\<tau> q1) \<and> ZR (set_type C) q1 {p'}\<close> 
+    with someI_ex[OF q1_ex] have X: \<open>\<exists>q. (q \<in> Q \<and> q  \<Rightarrow>^\<tau> q1) \<and> F (set_type C) q1 {p'}\<close> 
       by blast
     hence \<open>q1 \<in> weak_tau_succs Q \<and> {p'} = {p'}\<close>using weak_tau_succs_def by auto
     thus ?thesis  using n0_def strat q1_def by auto
@@ -384,7 +384,7 @@ proof -
   thus ?thesis using \<open>p = p1\<close> n0_def by auto
 qed
 
-lemma defSimNode_with_prefix_in_play: 
+lemma def_sim_pos_with_prefix_in_play: 
   assumes 
     \<open>A \<noteq> []\<close>
     \<open>p \<Rightarrow>$A p1\<close> 
@@ -515,7 +515,7 @@ proof (safe)
     then obtain A_play p0 where 
      gotoA: \<open>DefenderSimNode (last A) p0 (dsuccs_seq_rec (rev (butlast A)) {q}) # A_play
         \<in> plays_for_strategy f\<close> \<open>word_reachable_via_delay A p p0 p1\<close> 
-        using defSimNode_with_prefix_in_play \<open>p \<Rightarrow>$A p1\<close> 
+        using def_sim_pos_with_prefix_in_play \<open>p \<Rightarrow>$A p1\<close> 
         \<open>\<forall>a\<in>set A. a \<noteq> \<tau>\<close> \<open>A \<noteq> []\<close> assms(1,2) play_def play_hd by meson
     then obtain Q where Q_def: \<open>Q = dsuccs_seq_rec (rev (butlast A)) {q}\<close> by auto
     hence Q_all: \<open>\<forall>q' \<in> Q.  q \<Rightarrow>$(butlast A) q'\<close> using in_dsuccs_implies_word_reachable by auto
