Contrasimulation.thy
@@ -114,33 +114,33 @@ lemma symm_weak_sim_is_contrasim:
 
 subsection \<open>Intermediate Relation Mimicking Contrasim\<close>
 
-definition ZR :: "(('s \<Rightarrow> ('s set) \<Rightarrow> bool)) \<Rightarrow> ('s \<Rightarrow> ('s set) \<Rightarrow> bool)" where 
-\<open>ZR R p' Q' \<equiv> \<exists>p Q A. R p Q \<and> p \<Rightarrow>$A p' \<and> (\<forall>a \<in> set A. a \<noteq> \<tau>) \<and> Q' = (dsuccs_seq_rec (rev A) Q)\<close>
+definition F :: "(('s \<Rightarrow> ('s set) \<Rightarrow> bool)) \<Rightarrow> ('s \<Rightarrow> ('s set) \<Rightarrow> bool)" where 
+\<open>F R p' Q' \<equiv> \<exists>p Q A. R p Q \<and> p \<Rightarrow>$A p' \<and> (\<forall>a \<in> set A. a \<noteq> \<tau>) \<and> Q' = (dsuccs_seq_rec (rev A) Q)\<close>
 
 definition set_type :: "('s \<Rightarrow> 's \<Rightarrow> bool) \<Rightarrow> ('s \<Rightarrow> ('s set) \<Rightarrow> bool)" where 
 \<open>set_type R p Q \<equiv> \<exists>q. R p q \<and> Q = {q}\<close>
 
-lemma R_is_in_ZR : 
+lemma R_is_in_F_of_R : 
   assumes \<open>R p Q\<close>
-  shows \<open>ZR R p Q\<close>
+  shows \<open>F R p Q\<close>
 proof -
   have Q_cond: \<open>Q = dsuccs_seq_rec (rev []) Q\<close>  by simp 
   have p_cond: \<open>p \<Rightarrow>$[] p\<close> using steps.simps weak_step_seq.simps(1) by blast 
-  thus \<open>ZR R p Q\<close> using Q_cond ZR_def \<open>R p Q\<close>
+  thus \<open>F R p Q\<close> using Q_cond F_def \<open>R p Q\<close>
     by (metis bex_empty empty_set tau_tau)
 qed
 
-lemma ZR_C_guarantees_tau_succ:
+lemma F_of_C_guarantees_tau_succ:
   assumes 
     \<open>contrasim C\<close>
-    \<open>ZR (set_type C) p Q\<close>
+    \<open>F (set_type C) p Q\<close>
     \<open>p \<Rightarrow>^\<tau> p'\<close>
-  shows \<open>\<exists>q'. q' \<in> (weak_tau_succs Q) \<and> ZR (set_type C) q' {p'}\<close>
+  shows \<open>\<exists>q'. q' \<in> (weak_tau_succs Q) \<and> F (set_type C) q' {p'}\<close>
 proof -
   obtain p0 Q0 A q0
       where \<open>(set_type C) p0 Q0\<close> \<open>p0 \<Rightarrow>$A p\<close> \<open>\<forall>a \<in> set A. a \<noteq> \<tau>\<close> \<open>Q0 = {q0}\<close> 
         and Q_def: \<open>Q = (dsuccs_seq_rec (rev A) Q0)\<close> 
-      using ZR_def assms set_type_def by metis
+      using F_def assms set_type_def by metis
   hence \<open>C p0 q0\<close> using set_type_def by auto 
   have \<open>p0 \<Rightarrow>$(A@[\<tau>]) p'\<close> using \<open>p0 \<Rightarrow>$A p\<close>  \<open>p \<Rightarrow>^\<tau>  p'\<close> rev_seq_step_concat by auto
   hence word: \<open>p0 \<Rightarrow>$A p'\<close> 
@@ -148,26 +148,26 @@ proof -
   then obtain q' where \<open>q0 \<Rightarrow>$A q'\<close> \<open>C q' p'\<close> 
     using assms contrasim_def[of \<open>C\<close>] \<open>C p0 q0\<close> \<open>\<forall>a \<in> set A. a \<noteq> \<tau>\<close> by blast
   hence \<open>(set_type C) q' {p'}\<close> using set_type_def by auto
-  hence inZR: \<open>ZR (set_type C) q' {p'}\<close> using R_is_in_ZR  by auto
+  hence inF: \<open>F (set_type C) q' {p'}\<close> using R_is_in_F_of_R  by auto
   have \<open>q' \<in> weak_tau_succs (dsuccs_seq_rec (rev A) Q0)\<close> 
     using \<open>Q0 = {q0}\<close> \<open>q0 \<Rightarrow>$ A q'\<close>
     by (simp add: word_reachable_implies_in_dsuccs) 
   hence \<open>q' \<in> weak_tau_succs Q\<close> using Q_def by simp 
-  thus \<open>\<exists>q'. q' \<in> weak_tau_succs Q \<and> ZR (set_type C) q' {p'}\<close> using inZR by auto
+  thus \<open>\<exists>q'. q' \<in> weak_tau_succs Q \<and> F (set_type C) q' {p'}\<close> using inF by auto
 qed
 
-lemma ZR_C_guarantees_action_succ :
+lemma F_of_C_guarantees_action_succ :
  assumes 
     \<open>contrasim C\<close>
-    \<open>ZR (set_type C) p Q\<close>
+    \<open>F (set_type C) p Q\<close>
     \<open>p =\<rhd>a p'\<close>
     \<open>a \<noteq> \<tau>\<close>
-  shows \<open>dsuccs a Q \<noteq> {}  \<and> ZR (set_type C) p' (dsuccs a Q)\<close>
+  shows \<open>dsuccs a Q \<noteq> {}  \<and> F (set_type C) p' (dsuccs a Q)\<close>
 proof -
   obtain p0 Q0 A q0
     where \<open>(set_type C) p0 Q0\<close> \<open>p0 \<Rightarrow>$A p\<close> \<open>Q0 = {q0}\<close> \<open>\<forall>a \<in> set A. a \<noteq> \<tau> \<close> 
       and Q_def: \<open>Q = (dsuccs_seq_rec (rev A) Q0)\<close> 
-    using ZR_def assms set_type_def by metis
+    using F_def assms set_type_def by metis
   then obtain CS where CS_def: \<open>contrasim CS \<and> CS p0 q0\<close> 
     using assms set_type_def by (metis singleton_inject) 
   have notau: \<open>\<forall>a \<in> set (A@[a]). a \<noteq> \<tau>\<close> 
@@ -186,8 +186,8 @@ proof -
   hence \<open>q1 \<in> dsuccs_seq_rec (a#(rev A)) {q0}\<close> by auto
   hence \<open>q1 \<in> dsuccs a (dsuccs_seq_rec (rev A) {q0})\<close>  by auto
   hence notempty: \<open>q1 \<in> dsuccs a Q\<close> using Q_def \<open>Q0 = {q0}\<close> by auto
-  have \<open>ZR (set_type C) p' (dsuccs a Q)\<close> 
-    using in_dsuccs word ZR_def[of \<open>(set_type C)\<close>] \<open>(set_type C) p0 Q0\<close> 
+  have \<open>F (set_type C) p' (dsuccs a Q)\<close> 
+    using in_dsuccs word F_def[of \<open>(set_type C)\<close>] \<open>(set_type C) p0 Q0\<close> 
       \<open>Q0 = {q0}\<close> Q_def notau simp_dsuccs_seq_rev by meson
   with notempty show ?thesis by auto
 qed
